Phi_Logic_Programming_Reasoner/Phi_Logic_Programming_Reasoner.thy
@@ -1,0 +1,336 @@
+theory Phi_Logic_Programming_Reasoner
+  imports Main "HOL-Eisbach.Eisbach" "HOL-Eisbach.Eisbach_Tools"
+  keywords "no" "on" :: quasi_command
+    and "\<phi>reasoner" "\<phi>reasoner_ML" :: thy_decl % "ML"
+  abbrevs
+      "<premise>" = "\<^bold>p\<^bold>r\<^bold>e\<^bold>m\<^bold>i\<^bold>s\<^bold>e"
+  and "<simprem>" = "\<^bold>s\<^bold>i\<^bold>m\<^bold>p\<^bold>r\<^bold>e\<^bold>m"
+begin
+
+chapter \<open>\<phi> Logic Programming Reasoner\<close>
+
+text \<open>This is a reasoner based on logic programming like Prolog.
+  A reasoning state is represented as a Horn clause, like
+\<^prop>\<open>(Premise1 \<Longrightarrow> Premise2 \<Longrightarrow> Antecedent1)
+\<Longrightarrow> (Premise21 \<Longrightarrow> Premise22 \<Longrightarrow> Antecedent2)
+\<Longrightarrow> Conclusion\<close>.
+  The order of subgoals (like Antecedent1 and Antecedent2 above) is significant.
+  A previous subgoal may instantiate schematic variables in later subgoals.
+  Therefore, instead of subgoal which implies unorder,
+    following logic terminology we call these subgoals \textit{antecedent}.
+  The reasoner always processes antecedents in order.
+  \<close>
+
+
+section \<open>Preliminary Configure\<close>
+
+named_theorems useful \<open>theorems that will be *used* in the automatic proving,
+          which basically has the same effect as the using command.\<close>
+
+attribute_setup rotated = \<open>Scan.lift (Scan.optional Parse.int 1 -- Scan.optional Parse.int 0) >>
+  (fn (k,j) => Thm.rule_attribute [] (fn _ => Thm.permute_prems j k))\<close>
+  \<open>Enhanced version of the Pure.rotated\<close>
+
+attribute_setup TRY_THEN = \<open>(Scan.lift (Scan.optional (Args.bracks Parse.nat) 1) -- Attrib.thm
+      >> (fn (i, B) => Thm.rule_attribute [B] (fn _ => fn A => A RSN (i, B) handle THM _ => A)))
+    \<close> "resolution with rule, and do nothing if fail"
+
+ML_file \<open>library/cost_net.ML\<close>
+
+section \<open>The Reasoner\<close>
+
+
+definition "\<phi>Intro_Rule x = x"
+definition "\<phi>Elim_Rule x = x"
+
+ML_file_debug \<open>library/reasoner.ML\<close>
+
+attribute_setup \<phi>reason =
+\<open>let open Args Scan Parse 
+  fun read_prop_mode mode ctxt = Syntax.read_prop (Proof_Context.set_mode mode ctxt)
+  val read_prop_pattern = read_prop_mode Proof_Context.mode_pattern
+  val prop_pattern = Scan.repeat (Scan.peek (named_term o read_prop_pattern o Context.proof_of))
+in
+  (lift (option add |-- ((\<^keyword>\<open>!\<close> >> K ~2000000) || optional (Parse.int >> ~) ~100))
+      -- (optional (lift ($$$ "on") |-- prop_pattern) []
+       -- optional (lift ($$$ "if" |-- $$$ "no") |-- prop_pattern) [])
+        >> Nu_Reasoner.attr_add_intro)
+  || (lift del >> K Nu_Reasoner.attr_del_intro)
+end\<close>
+  \<open>Set introduction rules in \<phi> reasonser.
+   Syntax: \<phi>intro [add] <spur-of-the-rule> || \<phi>intro del\<close>
+
+attribute_setup \<phi>reason_elim =
+\<open>let open Args Scan Parse
+  fun read_prop_mode mode ctxt = Syntax.read_prop (Proof_Context.set_mode mode ctxt)
+  val read_prop_pattern = read_prop_mode Proof_Context.mode_pattern
+  val prop_pattern = Scan.repeat (Scan.peek (named_term o read_prop_pattern o Context.proof_of))
+in
+  (lift (option add |-- ((\<^keyword>\<open>!\<close> >> K ~2000000) || optional (Parse.int >> ~) ~100))
+      -- (optional (lift ($$$ "on") |-- prop_pattern) []
+       -- optional (lift ($$$ "no") |-- prop_pattern) [])
+        >> Nu_Reasoner.attr_add_elim)
+  || (lift del >> K Nu_Reasoner.attr_del_elim)
+end\<close>
+  \<open>Set elimduction rules in \<phi> reasonser.
+  Syntax: \<phi>reasoner_elim [add] <spur-of-the-rule> || \<phi>reasoner_elim del\<close>
+
+method_setup \<phi>reason = \<open>let open Scan Parse in
+  Method.sections [
+    Args.add >> K (Method.modifier (Nu_Reasoner.attr_add_intro (~100,([],[]))) \<^here>),
+    Args.del >> K (Method.modifier  Nu_Reasoner.attr_del_intro \<^here>)
+] >> (fn irules => fn ctxt => fn ths => Nu_Reasoner.reason_tac ctxt)
+end\<close>
+
+declare conjI[\<phi>reason] TrueI[\<phi>reason]
+
+
+section \<open>Facilities & Tools\<close>
+
+subsection \<open>General Structures\<close>
+
+subsubsection \<open>Mode\<close>
+
+text \<open>Modes are annotations of the automation. They are typically used specifically to determine
+  the modes of the automation method to be applied. For example, see the Premise tag.\<close>
+
+typedef mode = "UNIV :: nat set" ..
+
+consts MODE_NORMAL :: mode \<comment> \<open>A generically used tag of the meaning of `default, the most common'.\<close>
+consts MODE_SIMP :: mode \<comment> \<open>relating to simplifier or simplification\<close>
+consts MODE_COLLECT :: mode \<comment> \<open>relating to collection\<close>
+
+subsubsection \<open>Focus\<close>
+
+text \<open>A general technical tag used in the reasoning, usually represents the reasoning
+  currently focuses on certain part, certain target.\<close>
+
+definition FOCUS_TAG :: " 'a \<Rightarrow> 'a "  ("\<blangle> _ \<brangle>") where [iff]: "\<blangle> x \<brangle> = x"
+
+
+subsection \<open>Proof Obligation\<close>
+
+definition Premise :: "mode \<Rightarrow> bool \<Rightarrow> bool" where "Premise _ x = x"
+
+abbreviation Normal_Premise ("\<^bold>p\<^bold>r\<^bold>e\<^bold>m\<^bold>i\<^bold>s\<^bold>e _" [27] 26) where "Normal_Premise \<equiv> Premise MODE_NORMAL"
+abbreviation Simp_Premise ("\<^bold>s\<^bold>i\<^bold>m\<^bold>p\<^bold>r\<^bold>e\<^bold>m _" [27] 26) where "Simp_Premise \<equiv> Premise MODE_SIMP"
+abbreviation Proof_Obligation ("\<^bold>o\<^bold>b\<^bold>l\<^bold>i\<^bold>g\<^bold>a\<^bold>t\<^bold>i\<^bold>o\<^bold>n _" [27] 26) where "Proof_Obligation \<equiv> Premise MODE_COLLECT"
+
+text \<open>
+  The tag represents an ordinary proof obligation other than the internal-system terms
+    that have a specific meaning and purpose and can be inferred automatically.
+  Thus, the tag simply triggers a general prover to attempt to solve it automatically.
+
+  There are multiple strategies to handle them, depending on the difficulty of the problem
+    and more specifically the solving time that the situation can afford.
+
+  The \<^term>\<open>\<^bold>p\<^bold>r\<^bold>e\<^bold>m\<^bold>i\<^bold>s\<^bold>e P\<close> denotes the \<^prop>\<open>P\<close> should be solved by full power, without counting
+    the potential very long time of waiting. In the situation, user usually can interrupt
+    the computation.
+
+  The \<^term>\<open>\<^bold>s\<^bold>i\<^bold>m\<^bold>p\<^bold>r\<^bold>e\<^bold>m P\<close> suits for time-sensible situation because the reasoner only uses
+    light-weight strategies to attack the goal, like `clarsimp'. Many reasoning rules use
+    this strategy because the time-consuming computation is not affordable during the automatic process.
+
+  The \<^term>\<open>\<^bold>o\<^bold>b\<^bold>l\<^bold>i\<^bold>g\<^bold>a\<^bold>t\<^bold>i\<^bold>o\<^bold>n P\<close> is interesting. Once it is presented in a Horn clause, proofs of
+    any \<^term>\<open>\<^bold>p\<^bold>r\<^bold>e\<^bold>m\<^bold>i\<^bold>s\<^bold>e P'\<close> before this tag are delayed until the proof of this tag.
+  In fact, proof obligations (\<^prop>\<open>P'\<close>) are moved into \<^term>\<open>\<^bold>o\<^bold>b\<^bold>l\<^bold>i\<^bold>g\<^bold>a\<^bold>t\<^bold>i\<^bold>o\<^bold>n P\<close> to be \<^term>\<open>\<^bold>o\<^bold>b\<^bold>l\<^bold>i\<^bold>g\<^bold>a\<^bold>t\<^bold>i\<^bold>o\<^bold>n P \<and> P'\<close>
+    by using conjuncture.
+  This strategy is useful when \<^prop>\<open>P'\<close> has undetermined schematic variables while those
+    variables can be determined by later automatic reasoning (by the reasoning of later subgoals in
+    the Horn clause but early than the \<^term>\<open>\<^bold>o\<^bold>b\<^bold>l\<^bold>i\<^bold>g\<^bold>a\<^bold>t\<^bold>i\<^bold>o\<^bold>n P\<close> tag).
+
+  When the automatic solving consumes a lot of time, users can set the auto level down to
+    semi-auto (level 1) to suppress the automatic behavior and solve it manually. (TODO: by which command?)
+\<close>
+
+lemma Premise_I[intro!]: "P \<Longrightarrow> Premise mode P" unfolding Premise_def by simp
+lemma Premise_D: "Premise mode P \<Longrightarrow> P" unfolding Premise_def by simp
+lemma Premise_E[elim!]: "Premise mode P \<Longrightarrow> (P \<Longrightarrow> C) \<Longrightarrow> C" unfolding Premise_def by simp
+
+lemma Premise_Irew: "(P \<Longrightarrow> C) \<equiv> Trueprop (\<^bold>p\<^bold>r\<^bold>e\<^bold>m\<^bold>i\<^bold>s\<^bold>e P \<longrightarrow> C)" unfolding Premise_def atomize_imp .
+
+lemma Premise_True[\<phi>reason 5000]: "Premise mode True" unfolding Premise_def ..
+lemma [\<phi>reason 5000]:
+  "Premise mode P
+  \<Longrightarrow> Premise mode (Premise any_mode P)"
+  unfolding Premise_def .
+
+
+paragraph \<open>Internal Lemmas\<close>
+
+lemma contract_premise_true:
+  "(True \<Longrightarrow> Premise mode B) \<equiv> Trueprop (Premise mode B) "
+  by simp
+
+lemma contract_premise_imp:
+  "(A \<Longrightarrow> Premise mode B) \<equiv> Trueprop (Premise mode (A \<longrightarrow> B)) "
+  unfolding Premise_def atomize_imp .
+
+lemma contract_premise_all:
+  "(\<And>x. Premise mode (P x)) \<equiv> Trueprop ( Premise mode (\<forall>x. P x)) "
+  unfolding Premise_def atomize_all .
+
+lemma Premise_refl[\<phi>reason 2000 on \<open>Premise ?mode (?x = ?x)\<close>]:
+  "Premise mode (x = x)"
+  unfolding Premise_def ..
+
+
+
+subsection \<open>Cut\<close>
+
+text \<open>There are three kinds of cuts.
+  \<^item> Local Cut : If the priority of a rule is greater (or equal) than 1000, this rule
+      is a local cut in the sense the reasoning will not branch but only apply this rule instead
+      (apply the rule with maximum priority if there are multiple rules are local cut).
+  \<^item> Global Cut : If the priority is greater (or equal) than 1000_000, this rule is
+      a global cut that no backtrack will be applied before this.
+      It implies some achievement has been reached.
+      Thus the reasoner returns the latest global cut point when not all antecedents are solved.
+  \<^item> Ultimate Cut i.e. \<r>Success : It represents an ultimate success has been reached in the reasoning,
+      so the reasoner terminates and returns the Horn clause triggering \<r>Success.\<close>
+
+
+definition \<r>Cut :: bool where \<open>\<r>Cut = True\<close>
+
+text \<open>It triggers a (global) reasoning cut.\<close>
+
+lemma [iff, \<phi>reason 1000000]: \<open>\<r>Cut\<close> unfolding \<r>Cut_def ..
+
+
+
+
+definition \<r>Success :: bool where \<open>\<r>Success = True\<close>
+
+lemma \<r>Success_I[iff]: \<open>\<r>Success\<close> unfolding \<r>Success_def ..
+
+text \<open>Terminates the reasoning successfully and immediately\<close>
+
+\<phi>reasoner_ML \<r>Success 10000 (conclusion \<open>\<r>Success\<close>) = \<open>fn (ctxt,sequent) =>
+  raise Nu_Reasoner.Success (ctxt, @{thm \<r>Success_I} RS sequent)\<close>
+
+
+
+subsection \<open>Conversion\<close>
+
+definition Conv :: " 'a \<Rightarrow> 'a \<Rightarrow> bool " ("\<^bold>c\<^bold>o\<^bold>n\<^bold>v _ = _" [51,51] 50)
+  where "Conv origin obj \<longleftrightarrow> obj = origin"
+
+text \<open>\<^prop>\<open>\<^bold>c\<^bold>o\<^bold>n\<^bold>v A = B\<close> indicates the reasoner should convert \<^term>\<open>A\<close> into some \<^term>\<open>B\<close>.
+  Specific rules should be configured to reason those goals.\<close>
+
+
+
+subsubsection \<open>Matches\<close>
+
+definition Matches :: \<open>'a \<Rightarrow> 'a \<Rightarrow> bool\<close> where \<open>Matches _ _ = True\<close>
+
+text \<open>In the reasoning, a subgoal \<^prop>\<open>Matches pattern term\<close> is solved iff \<^term>\<open>pattern\<close>
+  matches \<^term>\<open>term\<close>. This subgoal is useful to restrict a rule to match certain pattern to be applied.\<close>
+
+lemma Matches_I: \<open>Matches pattern term\<close> unfolding Matches_def ..
+
+\<phi>reasoner_ML Matches 2000 (conclusion \<open>Matches ?pattern ?term\<close>) =
+  \<open>fn (ctxt, sequent) =>
+    let
+      val (\<^const>\<open>Trueprop\<close> $ (Const (\<^const_name>\<open>Matches\<close>,_) $ pattern $ term))
+            = Thm.major_prem_of sequent
+    in
+      if Pattern.matches (Proof_Context.theory_of ctxt) (pattern, term)
+      then Seq.single (ctxt, @{thm Matches_I} RS sequent)
+      else Seq.empty
+    end\<close>
+
+
+
+subsection \<open>Not Match\<close>
+
+lemma NO_MATCH_I: "NO_MATCH A B" unfolding NO_MATCH_def ..
+
+\<phi>reasoner_ML NO_MATCH 0 (conclusion "NO_MATCH ?A ?B") = \<open>
+  fn (ctxt,th) =>
+  case try Thm.major_prem_of th
+    of SOME (\<^const>\<open>Trueprop\<close> $ (Const (\<^const_name>\<open>NO_MATCH\<close>, _) $ a $ b)) =>
+        if Pattern.matches (Proof_Context.theory_of ctxt) (a,b)
+        then Seq.empty
+        else Seq.single (ctxt, @{thm NO_MATCH_I} RS th)
+     | _ => Seq.empty
+\<close>
+
+
+
+subsubsection \<open>Subgoal\<close>
+
+typedef "subgoal" = "UNIV :: nat set" ..
+
+consts TOP_GOAL :: "subgoal"
+
+definition SUBGOAL :: "subgoal \<Rightarrow> subgoal \<Rightarrow> bool" where "SUBGOAL ROOT NEW_GOAL = True"
+definition CHK_SUBGOAL :: "subgoal \<Rightarrow> bool" \<comment> \<open>Check whether the goal is solved\<close>
+  where "CHK_SUBGOAL X = True"
+definition SOLVE_SUBGOAL :: "subgoal \<Rightarrow> bool" where "SOLVE_SUBGOAL X = True"
+
+text \<open>The three tags provides a hierarchical subgoal environment.
+  \<^prop>\<open>SUBGOAL ROOT NEW_GOAL\<close> creates a new unique subgoal \<^term>\<open>NEW_GOAL\<close> under \<^term>\<open>ROOT\<close>.
+    \<^term>\<open>NEW_GOAL\<close> should be a schematic variable to be instantiated by the reasoner.
+  \<^prop>\<open>SOLVE_SUBGOAL GOAL\<close> marks the GOAL and all its subgoals solved.
+  \<^prop>\<open>CHK_SUBGOAL GOAL\<close> checks whether the GOAL is marked solved. If it is,
+    this proposition is rejected to be solved by the reasoner, causing any search path
+    assuming this proposition terminates. Therefore, no additional searches
+    assuming this proposition will continue once the subgoal is solved.
+
+  Once \<^term>\<open>GOAL\<close> is marked solved. Later \<^prop>\<open>SOLVE_SUBGOAL GOAL\<close> only succeeds on the
+    search path which marks this goal. Any branch irrelevant with the point of
+    the marking cannot mark the \<^term>\<open>GOAL\<close> again, and \<^prop>\<open>SOLVE_SUBGOAL GOAL\<close>
+    fails for them, causing those branches terminate.
+
+  The \<^term>\<open>TOP_GOAL\<close> can never be solved.\<close>
+
+lemma SUBGOAL_I[iff]: "SUBGOAL ROOT NEWGOAL" unfolding SUBGOAL_def ..
+lemma CHK_SUBGOAL_I[iff]: "CHK_SUBGOAL X" unfolding CHK_SUBGOAL_def ..
+lemma SOLVE_SUBGOAL_I[iff]: "SOLVE_SUBGOAL X" unfolding SOLVE_SUBGOAL_def ..
+
+ML_file \<open>library/Subgoal_Env.ML\<close>
+
+\<phi>reasoner_ML SUBGOAL 2000 (conclusion \<open>SUBGOAL ?ROOT ?NEWGOAL\<close>) = \<open>Subgoal_Env.subgoal\<close>
+\<phi>reasoner_ML CHK_SUBGOAL 2000 (conclusion \<open>CHK_SUBGOAL ?GOAL\<close>) = \<open>Subgoal_Env.chk_subgoal\<close>
+\<phi>reasoner_ML SOLVE_SUBGOAL 9999 (conclusion \<open>SOLVE_SUBGOAL ?GOAL\<close>) = \<open>Subgoal_Env.solve_subgoal\<close>
+
+definition GOAL_CTXT :: "bool \<Rightarrow> subgoal \<Rightarrow> prop"  ("_  \<^bold>@\<^bold>G\<^bold>O\<^bold>A\<^bold>L _" [2,1000] 2)
+  where [iff]: "GOAL_CTXT x _ \<equiv> Trueprop x"
+
+
+
+subsection \<open>Simplification & Rewrite\<close>
+
+definition Simplify :: " mode \<Rightarrow> 'a \<Rightarrow> 'a \<Rightarrow> bool "
+  where "Simplify setting result origin \<longleftrightarrow> result = origin"
+
+lemma [cong]: "A = A' \<Longrightarrow> Simplify s x A = Simplify s x A' "
+  unfolding Simplify_def by simp
+
+lemma Simplify_I[intro!]: "Simplify s A A" unfolding Simplify_def ..
+lemma Simplify_E[elim!]: "Simplify s A B \<Longrightarrow> (A = B \<Longrightarrow> C) \<Longrightarrow> C" unfolding Simplify_def by blast
+
+
+subsubsection \<open>Default Simplifier\<close>
+
+consts default_simp_setting :: mode
+
+abbreviation Default_Simplify :: " 'a \<Rightarrow> 'a \<Rightarrow> bool " ("\<^bold>s\<^bold>i\<^bold>m\<^bold>p\<^bold>l\<^bold>i\<^bold>f\<^bold>y _ : _" [1000,10] 9)
+  where "Default_Simplify \<equiv> Simplify default_simp_setting"
+
+\<phi>reasoner Default_Simplify 1000 (conclusion \<open>Default_Simplify ?x ?y\<close>)
+  = (simp, rule Simplify_I)
+  
+(* \<open>fn ctx =>
+  HEADGOAL (asm_simp_tac ctx) THEN
+  HEADGOAL (resolve0_tac @{thms Simplify_I})
+\<close> *)
+
+
+
+
+
+
+end
